Bdd/Compactify.lean
@@ -1,0 +1,209 @@
+import Bdd.Basic
+open List renaming Vector → Vec
+
+open Pointer
+
+namespace Compactify
+-- def compactify_helper {n m : Nat} (O : OBdd n m) (S : O.SubBdd) (ids : Vec (Option (Fin O.numPointers)) m) (nid : Fin O.numPointers) (new : Vec (Node n O.numPointers) O.numPointers) : Vec (Option (Fin O.numPointers)) m × Fin O.numPointers × Vec (Node n O.numPointers) O.numPointers × Pointer O.numPointers :=
+--   match S_def : S with
+--   | ⟨U, hU⟩ =>
+--     match U_root_def : U.1.root with
+--     | terminal b => ⟨ ids, nid, new, terminal b ⟩
+--     | node j =>
+--       match ids.get j with
+--       | none =>
+--         have U_def : U = S.1 := by rw [S_def]
+--         let ⟨ ids1, nid1, new1, l ⟩ := compactify_helper O ⟨(U.low  U_root_def), sorry⟩ ids  nid  new
+--         let ⟨ ids2, nid2, new2, h ⟩ := compactify_helper O ⟨(U.high U_root_def), sorry⟩ ids1 nid1 new1
+--         have : NeZero O.numPointers := by apply OBdd.instNeZeroNumPointers; rw [← U_def]; assumption
+--         ⟨ids2.set j (some nid2), nid2 + (Fin.ofNat' O.numPointers 1), new2.set nid2 ⟨O.1.heap[j].var, l, h⟩, node nid2⟩
+--       | some j' => ⟨ ids, nid, new, node j' ⟩
+-- termination_by S.1
+-- decreasing_by
+--   · exact oedge_of_low
+--   · exact oedge_of_high
+
+def compactify_helper {n m : Nat} (O : OBdd n m) (S : O.SubBdd) (ids : Vec (Option (Fin O.numPointers)) m) (nid : Fin O.numPointers) (new : Vec (Node n O.numPointers) O.numPointers) : Vec (Option (Fin O.numPointers)) m × Fin O.numPointers × Vec (Node n O.numPointers) O.numPointers × Pointer O.numPointers :=
+  match S_root_def : S.1.1.root with
+    | terminal b => ⟨ ids, nid, new, terminal b ⟩
+    | node j =>
+      match ids.get j with
+      | none =>
+        let ⟨ ids1, nid1, new1, l ⟩ := compactify_helper O (S.low  S_root_def) ids  nid  new
+        let ⟨ ids2, nid2, new2, h ⟩ := compactify_helper O (S.high S_root_def) ids1 nid1 new1
+        have : NeZero O.numPointers := OBdd.instNeZeroNumPointers S S_root_def
+        ⟨ ids2.set j (some nid2), nid2 + 1, new2.set nid2 ⟨O.1.heap[j].var, l, h⟩, node nid2 ⟩
+      | some j' => ⟨ ids, nid, new, node j' ⟩
+termination_by S.1
+decreasing_by
+  · exact oedge_of_low
+  · exact oedge_of_high
+
+def compactify' {n m : Nat} (O : OBdd n m) : Bdd n O.numPointers :=
+  match O_root_def : O.1.root with
+  | terminal b =>
+    have := isTerminal_iff_numPointer_eq_zero.mpr ⟨b, O_root_def⟩
+    ⟨this ▸ Vec.nil, terminal (Bool_of_numPointer_eq_zero O this)⟩
+  | node j =>
+    let ⟨ ids, nid, new, r ⟩ := compactify_helper O O.toSubBdd (Vec.replicate m none) ⟨0, OBdd.numPointers_gt_zero_of_Sub_root_eq_node (O.toSubBdd) O_root_def⟩ (Vec.replicate O.numPointers ⟨O.1.heap[j].var, (terminal false), (terminal false)⟩)
+    ⟨new, r⟩
+
+-- lemma compactify_helper_ordered {n m : Nat} (O : OBdd n m) (S : O.SubBdd) (ids : Vec (Option (Fin O.numPointers)) m) (nid : Fin O.numPointers) (new : Vec (Node n O.numPointers) O.numPointers) :
+--     (∀ j j', ids.get j = some j' → Bdd.Ordered ⟨new, node j'⟩) →
+--     let ⟨ _, _, new1, r ⟩ := compactify_helper O S ids nid new
+--     Bdd.Ordered ⟨new1, r⟩ := by
+--   intro h
+--   unfold compactify_helper
+--   simp only
+--   split
+--   next b heq => apply Ordered_of_terminal
+--   next j heq =>
+--     split
+--     next heqq =>
+--       simp only
+--       sorry
+--     next j' heqq => e
+
+lemma compactify_helper_spec {n m : Nat}
+    (O : OBdd n m) (S : O.SubBdd) (ids : Vec (Option (Fin O.numPointers)) m) (nid : Fin O.numPointers) (new : Vec (Node n O.numPointers) O.numPointers) (hp : Proper new):
+    ( ∀ j j',
+      ids.get j = some j' →
+      ∃ (r : Reachable O.1.heap O.1.root (node j)),
+        OBdd.HIsomorphic ⟨⟨O.1.heap, node j⟩, ordered_of_relevant O ⟨node j, r⟩⟩ ⟨⟨new, node j'⟩, Ordered_of_Proper hp⟩
+    ) →
+    let ⟨ ids1, nid1, new1, root ⟩ := compactify_helper O S ids nid new
+    ∃ (hp' : Proper new1),
+      (∀ j j',
+       ids1.get j = some j' →
+       ∃ (r : Reachable O.1.heap O.1.root (node j)),
+         OBdd.HIsomorphic ⟨⟨O.1.heap, node j⟩, ordered_of_relevant O ⟨node j, r⟩⟩ ⟨⟨new1, node j'⟩, Ordered_of_Proper hp'⟩
+      ) ∧ OBdd.HIsomorphic S.1 ⟨⟨new1, root⟩, Ordered_of_Proper hp'⟩ := by
+  intro h
+  unfold compactify_helper
+  split
+  next ids2 nid2 new2 root heq =>
+    split at heq
+    next b heqq =>
+      simp only [Prod.mk.injEq] at heq
+      rcases heq with ⟨heq1, heq2, heq3, heq4⟩
+      rw [← heq3, ← heq1, ← heq4]
+      use hp
+      constructor
+      · exact h
+      · exact OBdd.HIsomorphic_of_terminal heqq rfl
+    next r heqq =>
+      split at heq
+      next heqqq =>
+        split at heq
+        next ids0 nid0 new0 lh heqqqq =>
+          split at heq
+          next ids1 nid1 new1 rh heqqqqq =>
+          simp only [Prod.mk.injEq] at heq
+          rcases heq with ⟨heq1, heq2, heq3, heq4⟩
+          have hp2 : Proper new2 := by
+            apply Proper_of_all_indices_RespectsOrder
+            intro j
+            nth_rw 2 [← heq3]
+            cases decEq nid1 j with
+            | isFalse hf =>
+              rw [Vec.get_set_of_ne' hf]
+              sorry
+            | isTrue ht =>
+              rw [ht, Vec.get_set_same']
+              sorry
+          sorry
+      next j heqqq => sorry
+  --     have hp' : Proper new1 := by
+  --       sorry
+  --     sorry
+  -- next b heq =>
+  --   constructor
+  --   · constructor
+  --     · exact h
+  --     · exact OBdd.HIsomorphic_of_terminal heq rfl
+  --   · simpa
+  -- next j heq =>
+  --   constructor
+  --   case w =>
+  --     split
+  --     next heqq =>
+  --       simp only
+  --       apply Proper_of_all_indices_RespectsOrder
+  --       intro i
+  --       sorry
+  --     next j' heqq => exact hp
+  --   case h =>
+  --     constructor
+  --     · intro jj j' hjj'
+  --       sorry
+  --     · sorry
+    -- · sorry
+    -- · constructor
+    --   · sorry
+    --   · constructor
+    --     case w =>
+    --       split
+    --       next heqq =>
+    --         simp only
+    --         apply Ordered_of_low_high_ordered
+    --         · rw [Vec.get_set_same']
+    --           simp only
+    --           suffices Bdd.Ordered ⟨(compactify_helper O (S.low heq) ids nid new).2.2.1, (compactify_helper O (S.low heq) ids nid new).2.2.2⟩ by
+    --             rintro ⟨x, hx⟩ ⟨y, hy⟩ hxy
+    --             simp only [GraphEdge, Ordered] at hxy
+    --             simp only [Ordered] at hx hy
+    --             simp only [GraphMayPrecede, MayPrecede]
+    --             sorry
+    --           rcases (compactify_helper_spec O (S.low heq) ids nid new h hp).2 with ⟨hhh, _⟩
+    --           exact hhh
+    --         · sorry
+    --         · sorry
+    --         · sorry
+    --       next j' heqq =>
+    --         exact (h j j' heqq).2.1
+    --     case h => sorry
+    -- split
+    -- next heqq =>
+    --   simp only
+    --   sorry
+    -- next j' heqq => exact h j j' heqq
+
+
+lemma compactify_ordered {n m : Nat} {O : OBdd n m} : (compactify' O).Ordered := by
+  unfold compactify'
+  split
+  next b heq => apply Bdd.Ordered_of_terminal
+  next j heq =>
+    split
+    next x ids nid new root heqq => sorry
+
+--theorem compactify_spec {n m : Nat} {O : OBdd n m} : O.Isomorphic (compactify O) :=
+
+lemma compactify_preserves_reduced {n m : Nat} {O : OBdd n m} :
+    OBdd.Reduced O → OBdd.Reduced ⟨(compactify' O), compactify_ordered⟩ := by
+  sorry
+
+end Compactify
+-- #eval (example_not_reduced_bdd).numPointers
+-- #eval (example_bdd).numPointers
+
+#eval example_bdd
+#eval! Compactify.compactify' example_bdd
+-- theorem compactify_induction {n m : Nat} {O : OBdd n m} {motive : Bdd n O.numPointers → Prop}
+--     (one : (h : O.numPointers = 0) → motive ⟨h ▸ Vec.nil, terminal (Bool_of_numPointer_eq_zero O h)⟩)
+--     (two : ∀ (k : Nat), O.numPointers = k.succ → motive (compactify O)) :
+--     motive (compactify O) := by
+--   cases h : O.numPointers with
+--   | zero =>
+--     convert one h
+--     · unfold compactify
+--       simp
+--     rw [compactify.]
+--   | succ k => sorry
+
+-- def compactify {n m : Nat} (O : OBdd n m) : Bdd n O.numPointers :=
+--   match h : O.numPointers with
+--   | 0 => ⟨Vec.nil, terminal (Bool_of_numPointer_eq_zero O h)⟩
+--   | Nat.succ k =>
+--     let ⟨ ids, nid, new, r ⟩ := compactify_helper O O.toSubBdd (Vec.replicate m none) ⟨0, by linarith⟩ (Vec.replicate O.numPointers ⟨(O.1.heap.get ⟨0, lt_of_le_of_lt (show 0 ≤ k by linarith) sorry⟩).var, (terminal false), (terminal false)⟩)
+--     h ▸ ⟨new, r⟩
